cedar-lean/Cedar/Spec/PartialValue.lean
@@ -1,0 +1,67 @@
+/-
+ Copyright 2022-2023 Amazon.com, Inc. or its affiliates. All Rights Reserved.
+
+ Licensed under the Apache License, Version 2.0 (the "License");
+ you may not use this file except in compliance with the License.
+ You may obtain a copy of the License at
+
+      https://www.apache.org/licenses/LICENSE-2.0
+
+ Unless required by applicable law or agreed to in writing, software
+ distributed under the License is distributed on an "AS IS" BASIS,
+ WITHOUT WARRANTIES OR CONDITIONS OF ANY KIND, either express or implied.
+ See the License for the specific language governing permissions and
+ limitations under the License.
+-/
+
+import Cedar.Data.Map
+import Cedar.Spec.Ext.IPAddr
+import Cedar.Spec.ExtFun
+import Cedar.Spec.PartialExpr
+import Cedar.Spec.Value
+
+/-!
+This file defines Cedar partial values.
+-/
+
+namespace Cedar.Spec
+
+open Cedar.Data
+
+inductive PartialValue where
+  | value (v : Value)
+  | residual (r : PartialExpr)
+
+deriving instance Repr, DecidableEq, Inhabited for PartialValue
+
+def PartialValue.asPartialExpr (v : PartialValue) : PartialExpr :=
+  match v with
+  | .value v    => v.asPartialExpr
+  | .residual r => r
+
+/--
+  Like `PartialValue`, but cannot contain residual expressions which depend on
+  vars or entity data
+-/
+inductive RestrictedPartialValue where
+  | value (v : Value)
+  | residual (r : RestrictedPartialExpr)
+
+deriving instance Inhabited for RestrictedPartialValue
+
+def RestrictedPartialValue.asPartialExpr (v : RestrictedPartialValue) : PartialExpr :=
+  match v with
+  | .value v    => v.asPartialExpr
+  | .residual r => r.asPartialExpr
+
+def RestrictedPartialValue.asRestrictedPartialExpr (v : RestrictedPartialValue) : RestrictedPartialExpr :=
+  match v with
+  | .value v    => v.asRestrictedPartialExpr
+  | .residual r => r
+
+def RestrictedPartialValue.asPartialValue (v : RestrictedPartialValue) : PartialValue :=
+  match v with
+  | .value v    => .value v
+  | .residual r => .residual (r.asPartialExpr)
+
+end Cedar.Spec
